Ghost state - log of operations

ew.fst
@@ -1,145 +1,79 @@
 module Ew
 
 open FStar.List.Tot
-
-val get_id : #op:eqtype -> (nat * op) -> nat
-let get_id (id, _) = id
-
-val get_op : #op:eqtype -> (nat * op) -> op
-let get_op (_, op) = op
-
-val mem_id : #op:eqtype
-           -> id:nat
-           -> l:list (nat * op)
-           -> Tot (b:bool{(exists op. mem (id,op) l) <==> b=true})
-let rec mem_id n l =
-  match l with
-  |[] -> false
-  |(id,_)::xs -> (n = id) || mem_id n xs
-
-val unique_id : #op:eqtype 
-              -> l:list (nat * op)
-              -> Tot bool
-let rec unique_id l =
-  match l with
-  |[] -> true
-  |(id,_)::xs -> not (mem_id id xs) && unique_id xs
-
-val get_eve : #op:eqtype 
-            -> id:nat 
-            -> l:list (nat * op){unique_id l /\ mem_id id l}
-            -> Tot (s:(nat * op) {get_id s = id /\ mem s l})
-let rec get_eve id l =
-  match l with
-  |(id1, x)::xs -> if id = id1 then (id1, x) else get_eve id xs 
-
-val forallb : #a:eqtype
-            -> f:(a -> bool)
-            -> l:list a
-            -> Tot (b:bool{(forall e. mem e l ==> f e) <==> b = true})
-let rec forallb #a f l = 
-  match l with
-  |[] -> true
-  |hd::tl -> if f hd then forallb f tl else false
-
-val existsb : #a:eqtype
-            -> f:(a -> bool)
-            -> l:list a 
-            -> Tot (b:bool{(exists e. mem e l /\ f e) <==> b = true})
-let rec existsb #a f l =
-  match l with
-  |[] -> false
-  |hd::tl -> if f hd then true else existsb f tl
-
-val sorted : #op:eqtype
-           -> l:list(nat * op){unique_id l} -> bool
-let rec sorted #op l =
-  match l with
-  |[] -> true
-  |x::[] -> true
-  |x::xs -> forallb (fun (e:(nat * op)) -> fst x < fst e) xs && sorted xs
-
-val filter : #a:eqtype
-           -> f:(a -> bool)
-           -> l:list a
-           -> Tot (l1:list a {forall e. mem e l1 <==> mem e l /\ f e})
-let rec filter #a f l = 
-  match l with
-  |[] -> []
-  |hd::tl -> if f hd then hd::(filter f tl) else filter f tl
-
-/////////////////////////////////////////
+open FStar.Ghost
+open FStar.Seq.Base
+open FStar.Seq.Properties
 
 type op =
   |Enable
   |Disable
 
-///SEQUENTIAL DATA TYPE IMPLEMENTATION///
+type ew_st = nat & bool //concrete state of the enable-wins flag
+type st = ew_st & (erased (Seq.seq (ew_st & (nat (*id*) & op))))
 
-type s = bool
+val init : st
+let init = ((0, false), hide empty)
 
-let init = false
+val get_id : (nat * op) -> nat
+let get_id (id, o) = id
 
-val do : s -> (nat * op) -> s
-let do s op =
-  match op with
-  |(_,Enable) -> true
-  |(_,Disable) -> false
+let get_op (_, o) = o
 
-val spec : s1:s -> o1:(nat * op) -> o2:(nat * op) -> s
-let spec s1 o1 o2 =
-  match get_op o1, get_op o2 with
-  |Enable, Disable -> do (do s1 o2) o1
-  |_ -> do (do s1 o1) o2
+val get_val : st -> ew_st
+let get_val (c, _) = c
 
-val fold : st:s -> l:list (nat * op){unique_id l} -> Tot s (decreases l)
-let rec fold s l =
-  match l with
-  |[] -> s
-  |x::xs -> fold (do s x) xs
+val get_seq : st -> GTot (Seq.seq (ew_st * (nat * op)))
+let get_seq (st, seq) = (reveal seq)
 
-////////////MRDT IMPLEMENTATION////////////
+val get_st : (ew_st * (nat * op)) -> ew_st
+let get_st (st, o) = st
 
-type s' = nat * bool
+val get_init : c:st -> GTot ew_st
+let get_init c = 
+  if (length (get_seq c) > 0) then get_st (head (get_seq c)) else get_val c
 
-val init' : s'
-let init' = (0, false)
+val last_op : c:st{length (get_seq c) > 0} -> GTot (nat * op)
+let last_op c = get_op (last (get_seq c))
 
-let pre_cond_do' s o = true
+val inverse : c:st{length (get_seq c) > 0} -> GTot ew_st
+let inverse c = get_st (last (get_seq c))
 
-val do' : st:s' -> o:(nat * op) -> st1:s'{(get_op o = Enable <==> (st1 = (fst st + 1, true))) /\
-                                      (get_op o = Disable <==> (st1 = (fst st, false)))}
-let do' s' op =
+val st_i : c:st{length (get_seq c) > 0} -> i:nat{i < length (get_seq c)} -> GTot ew_st
+let st_i c i = (get_st (index (get_seq c) i))
+
+val op_i : c:st{length (get_seq c) > 0} -> i:nat{i < length (get_seq c)} -> GTot (nat * op)
+let op_i c i = (get_op (index (get_seq c) i))
+
+let pre_cond_do s op = true 
+
+val do : st:ew_st -> o:(nat * op) -> st1:ew_st{(get_op o = Enable <==> (st1 = (fst st + 1, true))) /\
+                                           (get_op o = Disable <==> (st1 = (fst st, false)))}
+let do s' op =
   match op with
   |(_,Enable) -> (fst s' + 1, true)
   |(_,Disable) -> (fst s', false)
 
-val tl : l:list(nat * op){l <> []} -> Tot (t:(nat * op){mem t l})
-let rec tl l =
-  match l with
-  |[x] -> x
-  |x::xs -> tl xs
+let valid_st (c:st) = 
+  (forall i. i < length (get_seq c) - 1 ==> do (st_i c i) (op_i c i) = (st_i c (i+1))) /\
+  (length (get_seq c) > 0 ==> get_val c = do (inverse c) (last_op c))
 
-val fold' : st:s' -> l:list (nat * op)
-          -> Pure s'
-            (requires unique_id l)
-            (ensures (fun r -> ((l <> [] /\ (forall e. mem e l ==> get_op e <> Disable)) ==> (fst r > fst st)) /\
-                             (fst r >= fst st) /\ (l <> [] /\ get_op (tl l) = Enable ==> (fst r > fst st)) /\
-                             (l = [] ==> r = st) /\
-                             ((snd r = true) <==> ((l = [] /\ snd st = true) \/ (l <> [] /\ get_op (tl l) = Enable))) /\
-                             (l <> [] /\ get_op (tl l) = Disable ==> snd r = false)))
-              (decreases l)
-let rec fold' s l =
-  match l with
-  |[] -> s
-  |x::xs -> fold' (do' s x) xs
+val lemma1 : c:st
+           -> Lemma (requires valid_st c /\ length (get_seq c) > 0)
+                   (ensures fst (get_init c) <= fst (inverse c))
+                   (decreases (length (get_seq c)))
+let rec lemma1 c =
+  match (length (get_seq c)) with
+  |0 -> ()
+  |1 -> ()
+  |_ -> lemma1 (inverse c, hide (slice (get_seq c) 0 (length (get_seq c) - 1)))
 
-val pre_cond_merge' : l:s' -> a:s' -> b:s' -> bool
-let pre_cond_merge' l a b = fst a >= fst l && fst b >= fst l
+val pre_cond_merge : l:ew_st -> a:ew_st -> b:ew_st -> bool
+let pre_cond_merge l a b = fst a >= fst l && fst b >= fst l
 
-val merge_flag : l:s'
-               -> a:s'{fst a >= fst l}
-               -> b:s'{fst b >= fst l}
+val merge_flag : l:ew_st
+               -> a:ew_st{fst a >= fst l}
+               -> b:ew_st{fst b >= fst l}
                -> Tot (b1:bool {(b1 = true <==> (snd a = true /\ snd b = true) \/ 
                                              (snd a = true /\ snd b = false /\ fst a > fst l) \/
                                              (snd b = true /\ snd a = false /\ fst b > fst l)) /\
@@ -157,123 +91,70 @@ let merge_flag l a b =
         else if af then ac - lc > 0
           else bc - lc > 0
 
-val merge' : l:s' 
-           -> a:s'
-           -> b:s'
-           -> Pure s'
-             (requires pre_cond_merge' l a b)
-             (ensures (fun r -> r = (fst a + fst b - fst l, merge_flag l a b)))
-let merge' l a b =
+val merge : l:ew_st
+          -> a:ew_st
+          -> b:ew_st
+          -> Pure ew_st (requires pre_cond_merge l a b)
+                       (ensures (fun r -> r = (fst a + fst b - fst l, merge_flag l a b)))
+let merge l a b =
   let c = fst a + fst b - fst l in
   let f = merge_flag l a b in
   c, f
 
-////////////////////////////////////////////
+//equivalence relation between 2 states
+val eq_m : a:ew_st -> b:ew_st -> bool
+let eq_m a b = a = b
 
-val eq : st:s -> st':s' -> bool
-let eq s s' = s = snd s'
+val prop_merge1 : l:st -> a:st -> b:st
+                -> Lemma (requires valid_st l /\ valid_st a /\ valid_st b /\ 
+                                  length (get_seq a) > 0 /\ length (get_seq b) > 0 /\
+                                  get_init a = get_init b /\ get_init a = get_val l /\ 
+                                  pre_cond_merge (get_val l) (get_val a) (get_val b))
+                         (ensures pre_cond_merge (get_val l) (inverse a) (inverse b) /\
+                                  (let m = merge (get_val l) (inverse a) (inverse b) in
+                                       eq_m (merge (get_val l) (get_val a) (get_val b)) 
+                                            (merge m (do m (last_op a)) (do m (last_op b)))))
+let prop_merge1 l a b = 
+  lemma1 a;
+  lemma1 b
 
-val eq_m : a:s' -> b:s' -> bool
-let eq_m a b = snd a = snd b
+val prop_merge2 : l:st -> a:st -> b:st
+                -> Lemma (requires valid_st l /\ valid_st a /\ valid_st b /\ 
+                                  length (get_seq a) = 0 /\ length (get_seq b) > 0 /\
+                                  get_val a = get_init b /\ get_val a = get_val l /\
+                                  pre_cond_merge (get_val l) (get_val a) (get_val b))
+                        (ensures pre_cond_merge (get_val l) (get_val a) (inverse b) /\
+                                 (let m = merge (get_val l) (get_val a) (inverse b) in
+                                      eq_m (merge (get_val l) (get_val a) (get_val b)) (do m (last_op b))))
+let prop_merge2 l a b = 
+  lemma1 b
 
-val prop_init : unit -> Lemma (ensures (eq init init'))
-let prop_init () = ()
+val prop_merge3 : l:st -> a:st -> b:st
+                -> Lemma (requires valid_st l /\ valid_st a /\ valid_st b /\ 
+                                  length (get_seq a) > 0 /\ length (get_seq b) = 0 /\
+                                  get_val b = get_init a /\ get_val b = get_val l /\
+                                  pre_cond_merge (get_val l) (get_val a) (get_val b))
+                        (ensures pre_cond_merge (get_val l) (inverse a) (get_val b) /\
+                                 (let m = merge (get_val l) (inverse a) (get_val b) in
+                                      eq_m (merge (get_val l) (get_val a) (get_val b)) (do m (last_op a))))
+let prop_merge3 l a b = 
+  lemma1 a
 
-val prop_equivalence : a:s' -> b:s' -> o:(nat * op)
-                     -> Lemma (requires (eq_m a b /\ pre_cond_do' a o /\ pre_cond_do' b o))
-                             (ensures (eq_m (do' a o) (do' b o)))
-let prop_equivalence a b o = ()
+val spec : (nat * bool) -> (nat * op) -> (nat * op) -> (nat * bool)
+let spec a o1 o2 =
+  match o1, o2 with
+  |(_, Enable), (_, Disable) -> do (do a o2) o1
+  |_ -> do (do a o1) o2
 
-val prop_do : st:s -> st':s' -> o:(nat * op)
-            -> Lemma (requires (eq st st'))
-                    (ensures (eq (do st o) (do' st' o)))
-let prop_do s s' op = ()
-
-val inverse : st:s' -> o:(nat * op) 
-            -> Pure (list s') 
-              (requires (get_op o = Enable ==> fst st > 0) /\
-                        (get_op o = Disable <==> snd st = false))
-              (ensures (fun r -> (forall e. mem e r ==> st = do' e o)))
-let inverse a o =
-  match o with
-  |(_, Enable) -> [(fst a - 1, true); (fst a - 1, false)]
-  |(_, Disable) -> [(fst a, false); (fst a, true)]
-
-val append : l1:list(nat * op) -> l2:list(nat * op)
-           -> Pure (list (nat * op))
-                  (requires (forall e. mem e l1 ==> not (mem_id (get_id e) l2)) /\
-                            unique_id l1 /\ unique_id l2)
-                  (ensures (fun r -> (forall e. mem e r <==> mem e l1 \/ mem e l2) /\ unique_id r /\
-                                  (l2 <> [] ==> tl r = tl l2)))
-                  (decreases %[l1;l2])
-let rec append l1 l2 =
-  match l1, l2 with
-  |[],[] -> []
-  |x::xs,_ -> x::(append xs l2)
-  |[],x::xs -> x::(append [] xs)
-
-val prop_merge1 : l:s' -> a:s' -> b:s' 
-                -> atr:list(nat * op) -> o1:(nat * op) 
-                -> btr:list(nat * op) -> o2:(nat * op) 
-                -> Lemma (requires (unique_id atr /\ unique_id btr /\ get_id o1 <> get_id o2 /\
-                                  (forall e. mem e atr ==> not (mem_id (get_id e) btr)) /\
-                                  not (mem_id (get_id o1) atr) /\ not (mem_id (get_id o1) btr) /\
-                                  not (mem_id (get_id o2) atr) /\ not (mem_id (get_id o2) btr) /\
-                                  a = fold' l (append atr [o1]) /\ b = fold' l (append btr [o2])))
-                        (ensures (forall ia ib. mem ia (inverse a o1) /\ mem ib (inverse b o2) ==>
-                                   (let merge_prefix = (merge' l ia ib) in 
-                                      ((merge' l a b) = (merge' merge_prefix (do' merge_prefix o1) (do' merge_prefix o2))))))
-let prop_merge1 l a b atr o1 btr o2 = ()
-
-val prop_merge2 : l:s' -> a:s' -> b:s' -> op1:(nat * op) -> op2:(nat * op)
-                -> Lemma (requires (a = do' l op1 /\ b = do' l op2 /\ get_id op1 <> get_id op2))
-                        (ensures (pre_cond_merge' l a b) /\
-                                 (forall sl. eq sl l ==> (eq (spec sl op1 op2) (merge' l a b))))
-let prop_merge2 l a b opa opb = ()
-
-(*)val prop_merge3 : l:s' -> a:s' -> atr:list(nat * op) -> o1:(nat * op)
-                -> Lemma (requires (unique_id atr /\ not (mem_id (get_id o1) atr) /\
-                                  (a = fold' l (append atr [o1])) /\
-                                  (forall e. mem e (inverse a o1) ==> e = fold' l atr)))
-                        (ensures (forall ia. mem ia (inverse a o1) ==>
-                                    (merge' l a l) = (merge' l ia (do' l o1))))
-let prop_merge3 l a atr o1 = ()*)
-
-val prop_merge4 : l:s' -> a:s' -> op1:(nat * op)
-                -> Lemma (requires (a = do' l op1))
-                        (ensures (pre_cond_merge' l a l) /\
-                                 (forall sl. eq sl l ==> (eq (do sl op1) (merge' l a l))))
-let prop_merge4 l a op1 = ()
-
-val idempotence : a:s'
-                -> Lemma (ensures (a = (merge' a a a)))
-let idempotence a = ()
-
-val commutativity : l:s' 
-                  -> a:s'
-                  -> b:s'
-                  -> Lemma (requires (exists atr btr. unique_id atr /\ unique_id btr /\ a = fold' l atr /\ b = fold' l btr))
-                          (ensures (merge' l b a = merge' l a b))
-let commutativity l a b = ()
-
-val associativity : l:s'
-                  -> a:s'
-                  -> b:s'
-                  -> c:s'
-                  -> Lemma (requires (exists atr btr ctr. unique_id atr /\ unique_id btr /\ unique_id ctr /\
-                                     a = fold' l atr /\ b = fold' l btr /\ c = fold' l ctr))
-                          (ensures (merge' l a (merge' l b c) = merge' l (merge' l a b) c))
-let associativity l a b c = ()
+val lem_spec : l:st -> a:st -> b:st
+             -> o1:(nat * op) -> o2:(nat * op)
+             -> Lemma (requires pre_cond_do (get_val l) o1 /\ pre_cond_do (get_val l) o2 /\ get_id o1 <> get_id o2 /\
+                               get_val a = do (get_val l) o1 /\ get_val b = do (get_val l) o2)
+                     (ensures pre_cond_merge (get_val l) (get_val a) (get_val b) /\ 
+                              eq_m (spec (get_val l) o1 o2) (merge (get_val l) (get_val a) (get_val b)))
+let lem_spec l a b o1 o2 = ()
 
 
-val prop_merge00 : l:s' -> a:s' -> b:s' -> op1:(nat * op) -> op2:(nat * op)
-                 -> Lemma (requires (a = do' l op1 /\ b = do' l op2 /\ get_id op1 <> get_id op2 /\
-                                    (exists atr btr. unique_id atr /\ unique_id btr /\
-                                    a = fold' l atr /\ b = fold' l btr)))
-                         (ensures (pre_cond_merge' l a b) /\
-                                  (forall sl. eq sl (merge' l a b) ==> 
-                                     (eq (spec sl op1 op2) (merge' (merge' l a b)
-                                                                   (do' (merge' l a b) op1) 
-                                                                   (do' (merge' l a b) op2)))))
 
-let prop_merge00 l a b opa opb = ()
+
+
