ictr.fst
@@ -1,212 +1,125 @@
 module Ictr
 
 open FStar.List.Tot
-
-val get_id : #op:eqtype -> (nat * op) -> nat
-let get_id (id, _) = id
-
-val get_op : #op:eqtype -> (nat * op) -> op
-let get_op (_, op) = op
-
-val mem_id : #op:eqtype
-           -> id:nat
-           -> l:list (nat * op)
-           -> Tot (b:bool{(exists op. mem (id,op) l) <==> b=true})
-let rec mem_id n l =
-  match l with
-  |[] -> false
-  |(id,_)::xs -> (n = id) || mem_id n xs
-
-val unique_id : #op:eqtype 
-              -> l:list (nat * op)
-              -> Tot bool
-let rec unique_id l =
-  match l with
-  |[] -> true
-  |(id,_)::xs -> not (mem_id id xs) && unique_id xs
-
-val get_eve : #op:eqtype 
-            -> id:nat 
-            -> l:list (nat * op){unique_id l /\ mem_id id l}
-            -> Tot (s:(nat * op) {get_id s = id /\ mem s l})
-let rec get_eve id l =
-  match l with
-  |(id1, x)::xs -> if id = id1 then (id1, x) else get_eve id xs 
-
-val forallb : #a:eqtype
-            -> f:(a -> bool)
-            -> l:list a
-            -> Tot (b:bool{(forall e. mem e l ==> f e) <==> b = true})
-let rec forallb #a f l = 
-  match l with
-  |[] -> true
-  |hd::tl -> if f hd then forallb f tl else false
-
-val existsb : #a:eqtype
-            -> f:(a -> bool)
-            -> l:list a 
-            -> Tot (b:bool{(exists e. mem e l /\ f e) <==> b = true})
-let rec existsb #a f l =
-  match l with
-  |[] -> false
-  |hd::tl -> if f hd then true else existsb f tl
-
-val sorted : #op:eqtype
-           -> l:list(nat * op){unique_id l} -> bool
-let rec sorted #op l =
-  match l with
-  |[] -> true
-  |x::[] -> true
-  |x::xs -> forallb (fun (e:(nat * op)) -> fst x < fst e) xs && sorted xs
-
-val filter : #a:eqtype
-           -> f:(a -> bool)
-           -> l:list a
-           -> Tot (l1:list a {forall e. mem e l1 <==> mem e l /\ f e})
-let rec filter #a f l = 
-  match l with
-  |[] -> []
-  |hd::tl -> if f hd then hd::(filter f tl) else filter f tl
-
-/////////////////////////////////////////
+open FStar.Ghost
+open FStar.Seq.Base
+open FStar.Seq.Properties
 
 type op =
-  |Inc
+  | Inc
 
-///SEQUENTIAL DATA TYPE IMPLEMENTATION///
+type ctr_st = nat //concrete state of the counter
+type st = ctr_st & (erased (Seq.seq (ctr_st & (nat (*id*) & op))))
 
-type s = nat
+val init : st
+let init = (0, hide empty)
 
-let init = 0
+val get_id : (nat * op) -> nat
+let get_id (id, o) = id
 
-val do : s -> (nat * op) -> s
-let do s (_, Inc) = s + 1
+let get_op (_, o) = o
 
-val spec : s1:s -> o1:(nat * op) -> o2:(nat * op) -> s
-let spec s1 o1 o2 =
-  do (do s1 o1) o2
+val get_val : st -> ctr_st
+let get_val (c, _) = c
 
-val fold : st:s -> l:list (nat * op){unique_id l} -> Tot s (decreases l)
-let rec fold s l =
-  match l with
-  |[] -> s
-  |x::xs -> fold (do s x) xs
+val get_seq : st -> GTot (Seq.seq (ctr_st * (nat * op)))
+let get_seq (st, seq) = (reveal seq)
 
-////////////MRDT IMPLEMENTATION////////////
+val get_st : (ctr_st * (nat * op)) -> ctr_st
+let get_st (st, o) = st
 
-type s' = nat
+val get_init : c:st -> GTot nat
+let get_init c = 
+  if (length (get_seq c) > 0) then get_st (head (get_seq c)) else get_val c
 
-val init' : nat
-let init' = 0
+val last_op : c:st{length (get_seq c) > 0} -> GTot (nat * op)
+let last_op c = get_op (last (get_seq c))
 
-let pre_cond_do' s o = true
+val inverse : c:st{length (get_seq c) > 0} -> GTot ctr_st
+let inverse c = get_st (last (get_seq c))
 
-val do' : st:s' -> (nat * op) -> r:s'
-let do' s' (_, Inc) = s' + 1
+val st_i : c:st{length (get_seq c) > 0} -> i:nat{i < length (get_seq c)} -> GTot ctr_st
+let st_i c i = (get_st (index (get_seq c) i))
 
-val fold' : st:s' -> l:list (nat * op){unique_id l} -> Tot (st':s' {(st' >= st) /\ (st' = st + length l)})
-            (decreases l)
-let rec fold' s l =
-  match l with
-  |[] -> s
-  |x::xs -> fold' (do' s x) xs
+val op_i : c:st{length (get_seq c) > 0} -> i:nat{i < length (get_seq c)} -> GTot (nat * op)
+let op_i c i = (get_op (index (get_seq c) i))
 
-val pre_cond_merge' : l:s' -> a:s' -> b:s' -> bool
-let pre_cond_merge' l a b = a >= l && b >= l
+let pre_cond_do s op = true 
 
-val merge' : l:s' 
-           -> a:s'
-           -> b:s'
-           -> Pure s'
-             (requires pre_cond_merge' l a b)
-             (ensures (fun r -> r = a + b - l))
-let merge' l a b =
+val do : c:ctr_st -> (nat * op) -> c1:ctr_st{c1 > c}
+let do c (_, Inc) = c + 1
+
+let valid_st (c:st) = 
+  (forall i. i < length (get_seq c) - 1 ==> do (st_i c i) (op_i c i) = (st_i c (i+1))) /\
+  (length (get_seq c) > 0 ==> get_val c = do (inverse c) (last_op c))
+
+val lemma1 : c:st
+           -> Lemma (requires valid_st c /\ length (get_seq c) > 0)
+                   (ensures get_init c <= inverse c)
+                   (decreases (length (get_seq c)))
+let rec lemma1 c =
+  match (length (get_seq c)) with
+  |0 -> ()
+  |1 -> ()
+  |_ -> lemma1 (inverse c, hide (slice (get_seq c) 0 (length (get_seq c) - 1)))
+
+val pre_cond_merge : l:ctr_st -> a:ctr_st -> b:ctr_st -> bool
+let pre_cond_merge l a b = a >= l && b >= l
+
+val merge : l:ctr_st -> a:ctr_st -> b:ctr_st
+           -> Pure ctr_st (requires pre_cond_merge l a b)
+                    (ensures (fun r -> r = a + b - l))
+let merge l a b =
   a + b - l
 
-////////////////////////////////////////////
-
-val eq : st:s -> st':s' -> bool
-let eq s s' = s = s'
-
-val eq_m : a:s' -> b:s' -> bool
+//equivalence relation between 2 states
+val eq_m : a:ctr_st -> b:ctr_st -> bool
 let eq_m a b = a = b
 
-val prop_init : unit -> Lemma (ensures (eq init init'))
-let prop_init () = ()
+val prop_merge1 : l:st -> a:st -> b:st
+                -> Lemma (requires valid_st l /\ valid_st a /\ valid_st b /\ 
+                                  length (get_seq a) > 0 /\ length (get_seq b) > 0 /\
+                                  get_init a = get_init b /\ get_init a = get_val l /\ 
+                                  pre_cond_merge (get_val l) (get_val a) (get_val b))
+                         (ensures pre_cond_merge (get_val l) (inverse a) (inverse b) /\
+                                  (let m = merge (get_val l) (inverse a) (inverse b) in
+                                       eq_m (merge (get_val l) (get_val a) (get_val b)) 
+                                            (merge m (do m (last_op a)) (do m (last_op b)))))
+let prop_merge1 l a b = 
+  lemma1 a;
+  lemma1 b
 
-val prop_equivalence : a:s' -> b:s' -> o:(nat * op)
-                     -> Lemma (requires (eq_m a b /\ pre_cond_do' a o /\ pre_cond_do' b o))
-                             (ensures (eq_m (do' a o) (do' b o)))
-let prop_equivalence a b o = ()
+val prop_merge2 : l:st -> a:st -> b:st
+                -> Lemma (requires valid_st l /\ valid_st a /\ valid_st b /\ 
+                                  length (get_seq a) = 0 /\ length (get_seq b) > 0 /\
+                                  get_val a = get_init b /\ get_val a = get_val l /\
+                                  pre_cond_merge (get_val l) (get_val a) (get_val b))
+                        (ensures pre_cond_merge (get_val l) (get_val a) (inverse b) /\
+                                 (let m = merge (get_val l) (get_val a) (inverse b) in
+                                      eq_m (merge (get_val l) (get_val a) (get_val b)) (do m (last_op b))))
+let prop_merge2 l a b = 
+  lemma1 b
 
-val prop_do : st:s -> st':s' -> o:(nat * op)
-            -> Lemma (requires (eq st st'))
-                    (ensures (eq (do st o) (do' st' o)))
-let prop_do s s' op = ()
+val prop_merge3 : l:st -> a:st -> b:st
+                -> Lemma (requires valid_st l /\ valid_st a /\ valid_st b /\ 
+                                  length (get_seq a) > 0 /\ length (get_seq b) = 0 /\
+                                  get_val b = get_init a /\ get_val b = get_val l /\
+                                  pre_cond_merge (get_val l) (get_val a) (get_val b))
+                        (ensures pre_cond_merge (get_val l) (inverse a) (get_val b) /\
+                                 (let m = merge (get_val l) (inverse a) (get_val b) in
+                                      eq_m (merge (get_val l) (get_val a) (get_val b)) (do m (last_op a))))
+let prop_merge3 l a b = 
+  lemma1 a
 
-val inverse : s:s'{s > 0} -> o:(nat * op) -> r:s'{s = do' r o}
-let inverse a o = a - 1
+val spec : nat -> (nat * op) -> (nat * op) -> nat
+let spec a o1 o2 =
+  do (do a o1) o2
 
-val append : l1:list(nat * op) -> l2:list(nat * op)
-           -> Pure (list (nat * op))
-                  (requires (forall e. mem e l1 ==> not (mem_id (get_id e) l2)) /\
-                            unique_id l1 /\ unique_id l2)
-                  (ensures (fun r -> (forall e. mem e r <==> mem e l1 \/ mem e l2) /\ unique_id r))
-                  (decreases %[l1;l2])
-let rec append l1 l2 =
-  match l1, l2 with
-  |[],[] -> []
-  |x::xs,_ -> x::(append xs l2)
-  |[],x::xs -> x::(append [] xs)
-
-val prop_merge1 : l:s' -> a:s' -> b:s' 
-                -> atr:list(nat * op) -> o1:(nat * op) 
-                -> btr:list(nat * op) -> o2:(nat * op) 
-                -> Lemma (requires (unique_id atr /\ unique_id btr /\ get_id o1 <> get_id o2 /\
-                                  (forall e. mem e atr ==> not (mem_id (get_id e) btr)) /\
-                                  not (mem_id (get_id o1) atr) /\ not (mem_id (get_id o1) btr) /\
-                                  not (mem_id (get_id o2) atr) /\ not (mem_id (get_id o2) btr) /\
-                                  a = fold' l (append atr [o1]) /\ b = fold' l (append btr [o2])))
-                        (ensures (let merge_prefix = (merge' l (inverse a o1) (inverse b o2)) in 
-                                      ((merge' l a b) = (merge' merge_prefix (do' merge_prefix o1) (do' merge_prefix o2)))))
-let prop_merge1 l a b atr_p o1 btr_p o2 = ()
-
-val prop_merge2 : l:s' -> a:s' -> b:s' -> op1:(nat * op) -> op2:(nat * op)
-                -> Lemma (requires (a = do' l op1 /\ b = do' l op2 /\ get_id op1 <> get_id op2))
-                        (ensures (pre_cond_merge' l a b) /\
-                                 (forall sl. eq sl l ==> (eq (spec sl op1 op2) (merge' l a b))))
-let prop_merge2 l a b opa opb = ()
-
-(*)val prop_merge3 : l:s' -> a:s' -> atr:list(nat * op) -> o1:(nat * op)
-                -> Lemma (requires (unique_id atr /\ (forall e. mem e atr ==> get_id o1 <> get_id e)) /\
-                                  (a = fold' l (append atr [o1])))
-                        (ensures (merge' l a l) = (merge' l (inverse a o1) (do' l o1) ))
-let prop_merge3 l a atr o1 = ()*)
-
-val prop_merge4 : l:s' -> a:s' -> op1:(nat * op)
-                -> Lemma (requires (a = do' l op1))
-                        (ensures (pre_cond_merge' l a l) /\
-                                 (forall sl. eq sl l ==> (eq (do sl op1) (merge' l a l))))
-let prop_merge4 l a op1 = ()
-
-val idempotence : a:s'
-                -> Lemma (ensures (a = (merge' a a a)))
-let idempotence a = ()
-
-val commutativity : l:s' 
-                  -> a:s'
-                  -> b:s'
-                  -> Lemma (requires (exists atr btr. a = fold' l atr /\ b = fold' l btr))
-                          (ensures (merge' l b a = merge' l a b))
-let commutativity l a b = ()
-
-val associativity : l:s'
-                  -> a:s'
-                  -> b:s'
-                  -> c:s'
-                  -> Lemma (requires (exists atr btr ctr. a = fold' l atr /\ b = fold' l btr /\ c = fold' l ctr))
-                          (ensures (merge' l a (merge' l b c) = merge' l (merge' l a b) c))
-let associativity l a b c = ()
-
-
+val lem_spec : l:st -> a:st -> b:st
+             -> o1:(nat * op) -> o2:(nat * op)
+             -> Lemma (requires pre_cond_do (get_val l) o1 /\ pre_cond_do (get_val l) o2 /\ get_id o1 <> get_id o2 /\
+                               get_val a = do (get_val l) o1 /\ get_val b = do (get_val l) o2)
+                     (ensures pre_cond_merge (get_val l) (get_val a) (get_val b) /\ 
+                              eq_m (spec (get_val l) o1 o2) (merge (get_val l) (get_val a) (get_val b)))
+let lem_spec l a b o1 o2 = ()
 
